theory/JITFlattern_aux_l_jump.thy
@@ -62,42 +62,71 @@ proof(induct lt arbitrary: l1 l_pc1 l_jump1 l l_pc l_jump)
     then obtain l2' l_pc2' l_jump2' where b0:"jitflat_bpf [a] (l1,l_pc1,l_jump1) = (l2',l_pc2',l_jump2') \<and> jitflat_bpf lt (l2',l_pc2',l_jump2') = (l,l_pc,l_jump)" by auto
 
     hence "l_jump2' = update_l_jump a l_pc1 l_jump1" using jitflat_bpf.elims by force 
-    hence b1:"l_jump2' = (let (num,off,l_bin0) = a in  if (\<exists> src dst. x64_decode 0 l_bin0 = Some(3, Pcmpq_rr src dst)) then l_jump1@ [(of_nat (length l_pc1), of_nat (length l_pc1) + off)] else l_jump1)" using update_l_jump_def by simp
+    hence b1:"l_jump2' = (let (num,off,l_bin0) = a in if (\<exists> d. x64_decode 0 l_bin0 = Some(5, Pcall_i d)) then l_jump1@ [(of_nat (length l_pc1), off)]
+      else if (\<exists> src dst. x64_decode 0 l_bin0 = Some(3, Pcmpq_rr src dst)) then l_jump1@ [(of_nat (length l_pc1), of_nat (length l_pc1) + off)] else l_jump1)" using update_l_jump_def by simp
     thus ?case
-    proof(cases "\<not>(\<exists> src dst. x64_decode 0 (snd (snd a)) = Some(3, Pcmpq_rr src dst))")
+    proof(cases "(\<exists> d. x64_decode 0 (snd (snd a)) = Some(5, Pcall_i d))")
       case True
-      have b2_1:"l_jump2' = l_jump1" using b1 True  by (smt (verit, best) case_prod_conv split_pairs)
-      have b2_2:"length l_pc2' = length l_pc1 + 1" using b0 l_pc_length_prop by force 
-      hence "\<forall> x. x < length l_pc1 \<longrightarrow> x < length l_pc2'" by auto
-      hence "is_increase_list l_jump2' l_pc2'" using assm0 is_increase_list_def b2_1 by simp
-      hence "is_increase_list l_jump l_pc" using b0 Cons.hyps by blast 
-      then show ?thesis by simp
+      have b2_0:"l_jump2' = l_jump1@ [(of_nat (length l_pc1), (fst (snd a)))]" 
+          using True b1 by (smt (verit, ccfv_threshold) old.prod.case prod.collapse) 
+        hence b3:"\<forall> idx1 idx2. idx1<idx2 \<and> idx1\<ge>0 \<and> idx2 < length l_jump1 \<longrightarrow> fst (l_jump2'!idx1) < fst (l_jump2'!idx2)" using b2_0 assm0
+          by (simp add: is_increase_list_def nth_append)  
+        have b4:"nat (fst (l_jump2'!(length l_jump1))) = (length l_pc1)" using b2_0 by simp
+        have b5:"(\<forall> idx. idx \<ge>0 \<and> idx < length l_jump1 \<longrightarrow> nat (fst (l_jump1!idx)) < (length l_pc1))"
+          using assm0 is_increase_list_def by blast 
+        hence "(\<forall> idx. idx \<ge>0 \<and> idx < length l_jump1 \<longrightarrow> (fst (l_jump1!idx)) < (fst (l_jump2'!(length l_jump1))))"
+          using b4 b5 by (metis zless_nat_conj) 
+        hence b7_1:"(\<forall> idx. idx \<ge>0 \<and> idx < length l_jump1 \<longrightarrow> (fst (l_jump2'!idx)) < (fst (l_jump2'!(length l_jump1))))" by (simp add: b2_0 nth_append) 
+        hence b7:"(\<forall> idx1 idx2. idx1<idx2 \<and> idx1\<ge>0 \<and> idx2 < length l_jump2' \<longrightarrow> fst (l_jump2'!idx1) < fst (l_jump2'!idx2))" 
+          using b7_1 by (metis (no_types, lifting) One_nat_def Suc_eq_plus1 b2_0 b3 length_append less_SucE list.size(3) list.size(4)) 
+  
+        have "(\<forall> idx. idx \<ge>0 \<and> idx < length l_jump1 \<longrightarrow> nat (fst (l_jump1!idx)) < (length l_pc2'))"
+          using b5 by (metis b0 l_pc_length_prop trans_less_add2) 
+        hence b6:"(\<forall> idx. idx \<ge>0 \<and> idx < length l_jump2' \<longrightarrow> nat (fst (l_jump2'!idx)) < (length l_pc2'))"
+          by (smt (verit, ccfv_SIG) One_nat_def add.commute b0 b2_0 b4 l_pc_length_prop length_append less_Suc_eq list.size(3) list.size(4) nth_append plus_1_eq_Suc) 
+            
+        hence "is_increase_list l_jump2' l_pc2'"
+          using b6 b7 is_increase_list_def by simp
+        then show ?thesis using b0 Cons by blast
     next
       case False
-      have b2_0:"l_jump2' = l_jump1@ [(of_nat (length l_pc1), of_nat (length l_pc1) + (fst (snd a)))]" 
-        using False b1 by (smt (verit, ccfv_threshold) old.prod.case prod.collapse) 
-      hence b3:"\<forall> idx1 idx2. idx1<idx2 \<and> idx1\<ge>0 \<and> idx2 < length l_jump1 \<longrightarrow> fst (l_jump2'!idx1) < fst (l_jump2'!idx2)" using b2_0 assm0
-        by (simp add: is_increase_list_def nth_append)  
-      have b4:"nat (fst (l_jump2'!(length l_jump1))) = (length l_pc1)" using b2_0 by simp
-      have b5:"(\<forall> idx. idx \<ge>0 \<and> idx < length l_jump1 \<longrightarrow> nat (fst (l_jump1!idx)) < (length l_pc1))"
-        using assm0 is_increase_list_def by blast 
-      hence "(\<forall> idx. idx \<ge>0 \<and> idx < length l_jump1 \<longrightarrow> (fst (l_jump1!idx)) < (fst (l_jump2'!(length l_jump1))))"
-        using b4 b5 by (metis zless_nat_conj) 
-      hence b7_1:"(\<forall> idx. idx \<ge>0 \<and> idx < length l_jump1 \<longrightarrow> (fst (l_jump2'!idx)) < (fst (l_jump2'!(length l_jump1))))" by (simp add: b2_0 nth_append) 
-      hence b7:"(\<forall> idx1 idx2. idx1<idx2 \<and> idx1\<ge>0 \<and> idx2 < length l_jump2' \<longrightarrow> fst (l_jump2'!idx1) < fst (l_jump2'!idx2))" 
-        using b7_1 by (metis (no_types, lifting) One_nat_def Suc_eq_plus1 b2_0 b3 length_append less_SucE list.size(3) list.size(4)) 
-
-      have "(\<forall> idx. idx \<ge>0 \<and> idx < length l_jump1 \<longrightarrow> nat (fst (l_jump1!idx)) < (length l_pc2'))"
-        using b5 by (metis b0 l_pc_length_prop trans_less_add2) 
-      hence b6:"(\<forall> idx. idx \<ge>0 \<and> idx < length l_jump2' \<longrightarrow> nat (fst (l_jump2'!idx)) < (length l_pc2'))"
-        by (smt (verit, ccfv_SIG) One_nat_def add.commute b0 b2_0 b4 l_pc_length_prop length_append less_Suc_eq list.size(3) list.size(4) nth_append plus_1_eq_Suc) 
-          
-      hence "is_increase_list l_jump2' l_pc2'"
-        using b6 b7 is_increase_list_def by simp
-      then show ?thesis using b0 Cons by blast
+      have b1_1:"\<not>(\<exists> d. x64_decode 0 (snd (snd a)) = Some(5, Pcall_i d))" using False by simp
+      then show ?thesis
+      proof(cases "\<not>(\<exists> src dst. x64_decode 0 (snd (snd a)) = Some(3, Pcmpq_rr src dst))")
+      case True
+        have b2_1:"l_jump2' = l_jump1" using b1 True b1_1 by (smt (verit, best) case_prod_conv split_pairs)
+        have b2_2:"length l_pc2' = length l_pc1 + 1" using b0 l_pc_length_prop by force 
+        hence "\<forall> x. x < length l_pc1 \<longrightarrow> x < length l_pc2'" by auto
+        hence "is_increase_list l_jump2' l_pc2'" using assm0 is_increase_list_def b2_1 by simp
+        hence "is_increase_list l_jump l_pc" using b0 Cons.hyps by blast 
+        then show ?thesis by simp
+      next
+        case False
+        have b2_0:"l_jump2' = l_jump1@ [(of_nat (length l_pc1), of_nat (length l_pc1) + (fst (snd a)))]" 
+          using False b1 b1_1 by (smt (verit, ccfv_threshold) old.prod.case prod.collapse) 
+        hence b3:"\<forall> idx1 idx2. idx1<idx2 \<and> idx1\<ge>0 \<and> idx2 < length l_jump1 \<longrightarrow> fst (l_jump2'!idx1) < fst (l_jump2'!idx2)" using b2_0 assm0
+          by (simp add: is_increase_list_def nth_append)  
+        have b4:"nat (fst (l_jump2'!(length l_jump1))) = (length l_pc1)" using b2_0 by simp
+        have b5:"(\<forall> idx. idx \<ge>0 \<and> idx < length l_jump1 \<longrightarrow> nat (fst (l_jump1!idx)) < (length l_pc1))"
+          using assm0 is_increase_list_def by blast 
+        hence "(\<forall> idx. idx \<ge>0 \<and> idx < length l_jump1 \<longrightarrow> (fst (l_jump1!idx)) < (fst (l_jump2'!(length l_jump1))))"
+          using b4 b5 by (metis zless_nat_conj) 
+        hence b7_1:"(\<forall> idx. idx \<ge>0 \<and> idx < length l_jump1 \<longrightarrow> (fst (l_jump2'!idx)) < (fst (l_jump2'!(length l_jump1))))" by (simp add: b2_0 nth_append) 
+        hence b7:"(\<forall> idx1 idx2. idx1<idx2 \<and> idx1\<ge>0 \<and> idx2 < length l_jump2' \<longrightarrow> fst (l_jump2'!idx1) < fst (l_jump2'!idx2))" 
+          using b7_1 by (metis (no_types, lifting) One_nat_def Suc_eq_plus1 b2_0 b3 length_append less_SucE list.size(3) list.size(4)) 
+  
+        have "(\<forall> idx. idx \<ge>0 \<and> idx < length l_jump1 \<longrightarrow> nat (fst (l_jump1!idx)) < (length l_pc2'))"
+          using b5 by (metis b0 l_pc_length_prop trans_less_add2) 
+        hence b6:"(\<forall> idx. idx \<ge>0 \<and> idx < length l_jump2' \<longrightarrow> nat (fst (l_jump2'!idx)) < (length l_pc2'))"
+          by (smt (verit, ccfv_SIG) One_nat_def add.commute b0 b2_0 b4 l_pc_length_prop length_append less_Suc_eq list.size(3) list.size(4) nth_append plus_1_eq_Suc) 
+            
+        hence "is_increase_list l_jump2' l_pc2'"
+          using b6 b7 is_increase_list_def by simp
+        then show ?thesis using b0 Cons by blast
+      qed
     qed
   qed
-
+    
 lemma l_jump_is_distinct:"is_increase_list l_jump1 l_pc1 \<Longrightarrow> jitflat_bpf lt (l1, l_pc1, l_jump1) = (l_bin,l_pc,l_jump) \<Longrightarrow> distinct (map fst l_jump1) \<Longrightarrow> distinct (map fst l_jump)"
 proof(induct lt arbitrary: l1 l_pc1 l_jump1 l_bin l_pc l_jump)
   case Nil
@@ -112,36 +141,57 @@ next
   then obtain l2' l_pc2' l_jump2' where b0:"jitflat_bpf [a] (l1, l_pc1, l_jump1) = (l2', l_pc2', l_jump2') \<and> 
          jitflat_bpf lt (l2', l_pc2', l_jump2') = (l_bin,l_pc,l_jump)" by auto
   hence "l_jump2' = update_l_jump a l_pc1 l_jump1" using jitflat_bpf.elims by force 
-  hence b1:"l_jump2' = (let (num,off,l_bin0) = a in  if (\<exists> src dst. x64_decode 0 l_bin0 = Some(3, Pcmpq_rr src dst)) then l_jump1@ [(of_nat (length l_pc1), of_nat (length l_pc1) + off)] else l_jump1)" using update_l_jump_def by simp
+  hence b1:"l_jump2' = (let (num,off,l_bin0) = a in if (\<exists> d. x64_decode 0 l_bin0 = Some(5, Pcall_i d)) then l_jump1@ [(of_nat (length l_pc1),off)] 
+  else if (\<exists> src dst. x64_decode 0 l_bin0 = Some(3, Pcmpq_rr src dst)) then l_jump1@ [(of_nat (length l_pc1), of_nat (length l_pc1) + off)] else l_jump1)" using update_l_jump_def by simp
   thus ?case
-  proof(cases "\<not>(\<exists> src dst. x64_decode 0 (snd (snd a)) = Some(3, Pcmpq_rr src dst))")
+  proof(cases "\<exists> d. x64_decode 0 (snd (snd a)) = Some(5, Pcall_i d)")
     case True
-    have b2_1:"l_jump2' = l_jump1" using b1 True  by (smt (verit, best) case_prod_conv split_pairs)
-    hence b2:"distinct (map fst l_jump2')" using a1 by simp
-    have "is_increase_list l_jump2' l_pc2'" using  l_jump_elem_increases a3 b0 by blast
-    hence "distinct (map fst l_jump)" using b0 b1 b2 Cons b2_1 by blast
-    then show ?thesis using a1 by simp
-  next
-    case False
-    have b2_0:"l_jump2' = l_jump1@ [(of_nat (length l_pc1), of_nat (length l_pc1) + (fst (snd a)))]" 
-      using False b1 by (smt (verit, ccfv_threshold) old.prod.case prod.collapse) 
-    hence " (\<forall> idx. idx \<ge>0 \<and> idx < length l_jump1 \<longrightarrow> nat (fst (l_jump1!idx)) <  (length l_pc1))" using b0 False a3 l_jump_elem_increases a3 b0 is_increase_list_def by blast
+    have b2_0:"l_jump2' = l_jump1@ [(of_nat (length l_pc1), (fst (snd a)))]" 
+        using True b1 by (smt (verit, ccfv_threshold) old.prod.case prod.collapse) 
+    hence " (\<forall> idx. idx \<ge>0 \<and> idx < length l_jump1 \<longrightarrow> nat (fst (l_jump1!idx)) <  (length l_pc1))" using b0 True a3 l_jump_elem_increases a3 b0 is_increase_list_def by blast
     hence b2_1:" (\<forall> idx. idx \<ge>0 \<and> idx < length l_jump1 \<longrightarrow> nat (fst (l_jump1!idx)) \<noteq>  (length l_pc1))" by fastforce
     have b2_2:"nat(of_nat (length l_pc1)) = (length l_pc1)" by auto
     hence "\<forall> elem1 elem2. (elem1,elem2) \<in> set l_jump1 \<longrightarrow> elem1 \<noteq> of_nat (length l_pc1)" using b2_1 b2_2
-      by (metis eq_fst_iff in_set_conv_nth le0) 
+        by (metis eq_fst_iff in_set_conv_nth le0) 
     hence "\<forall> elem1. elem1 \<in> set (map fst l_jump1) \<longrightarrow> elem1 \<noteq> of_nat (length l_pc1)" by auto
-    
+      
     hence "distinct ((map fst l_jump1) @ [of_nat (length l_pc1)])" using Cons.prems(3) by auto 
     hence b2:"distinct (map fst l_jump2')" using b2_0 by simp
     then show ?thesis using Cons b2 b0 l_jump_elem_increases by blast 
+  next
+    case False
+    have b1_1:"\<not>(\<exists> d. x64_decode 0 (snd (snd a)) = Some(5, Pcall_i d))" using False by simp
+    then show ?thesis
+    proof(cases "\<not>(\<exists> src dst. x64_decode 0 (snd (snd a)) = Some(3, Pcmpq_rr src dst))")
+      case True
+      have b2_1:"l_jump2' = l_jump1" using b1 True b1_1 by (smt (verit, best) case_prod_conv split_pairs)
+      hence b2:"distinct (map fst l_jump2')" using a1 by simp
+      have "is_increase_list l_jump2' l_pc2'" using  l_jump_elem_increases a3 b0 by blast
+      hence "distinct (map fst l_jump)" using b0 b1 b2 Cons b2_1 by blast
+      then show ?thesis using a1 by simp
+    next
+      case False
+      have b2_0:"l_jump2' = l_jump1@ [(of_nat (length l_pc1), of_nat (length l_pc1) + (fst (snd a)))]" 
+        using False b1 b1_1 by (smt (verit, ccfv_threshold) old.prod.case prod.collapse) 
+      hence " (\<forall> idx. idx \<ge>0 \<and> idx < length l_jump1 \<longrightarrow> nat (fst (l_jump1!idx)) <  (length l_pc1))" using b0 False a3 l_jump_elem_increases a3 b0 is_increase_list_def by blast
+      hence b2_1:" (\<forall> idx. idx \<ge>0 \<and> idx < length l_jump1 \<longrightarrow> nat (fst (l_jump1!idx)) \<noteq>  (length l_pc1))" by fastforce
+      have b2_2:"nat(of_nat (length l_pc1)) = (length l_pc1)" by auto
+      hence "\<forall> elem1 elem2. (elem1,elem2) \<in> set l_jump1 \<longrightarrow> elem1 \<noteq> of_nat (length l_pc1)" using b2_1 b2_2
+        by (metis eq_fst_iff in_set_conv_nth le0) 
+      hence "\<forall> elem1. elem1 \<in> set (map fst l_jump1) \<longrightarrow> elem1 \<noteq> of_nat (length l_pc1)" by auto
+      
+      hence "distinct ((map fst l_jump1) @ [of_nat (length l_pc1)])" using Cons.prems(3) by auto 
+      hence b2:"distinct (map fst l_jump2')" using b2_0 by simp
+      then show ?thesis using Cons b2 b0 l_jump_elem_increases by blast 
+    qed
   qed
-qed
+ qed
 
 
-lemma flattern_jump_index_easy:
+lemma flattern_jump_index_easy_1:
   "jitflat_bpf lt (l1,l_pc1,l_jump1) = (l_bin,l_pc,l_jump) \<Longrightarrow>
   lt!(unat pc) = (num,off,l) \<Longrightarrow>
+  (\<exists> src dst. x64_decode 0 l = Some(3, Pcmpq_rr src dst)) \<Longrightarrow>
   find_target_pc_in_l_pc l_jump (of_nat(length(l_pc1))+uint pc) = Some npc \<Longrightarrow>
   lt \<noteq> [] \<Longrightarrow>
   pc = 0 \<Longrightarrow>
@@ -155,7 +205,8 @@ proof-
   a3:"lt \<noteq> []" and
   a4:"pc = 0" and
   a5:"distinct (map fst l_jump1)" and
-  a6:"is_increase_list l_jump1 l_pc1"
+  a6:"is_increase_list l_jump1 l_pc1" and
+  an:"(\<exists> src dst. x64_decode 0 l = Some(3, Pcmpq_rr src dst))"
   let "?xs" = "tl lt"
   let "?len" = "(length(l_pc1))"
   have a7:"(num,off,l)#?xs = lt" using a1 a3 a4
@@ -173,39 +224,161 @@ proof-
   hence b2:"(int ?len,npc) \<in> set l_jump" using a2 a4 b1 search_l_jump by auto 
    (* by (metis bot_nat_0.extremum_strict in_set_conv_nth list.size(3) list_in_list.simps(1) list_in_list.simps(2) list_in_list_implies_set_relation) *)
   have b3:"update_l_jump (num,off,l) l_pc l_jump = (
-  if (\<exists> src dst. x64_decode 0 l = Some(3, Pcmpq_rr src dst)) then l_jump@ [(of_nat (length l_pc), of_nat (length l_pc) + off)]
+  if (\<exists> d. x64_decode 0 l = Some(5, Pcall_i d)) then l_jump@ [(of_nat (length l_pc), off)]
+  else if (\<exists> src dst. x64_decode 0 l = Some(3, Pcmpq_rr src dst)) then l_jump@ [(of_nat (length l_pc), of_nat (length l_pc) + off)]
   else l_jump)" 
     apply(unfold update_l_jump_def Let_def,simp_all) done
   have b4:"l_jump \<noteq> []" using a2 by auto
   thus ?thesis
-  proof(cases "(\<exists> src dst. x64_decode 0 l = Some(3, Pcmpq_rr src dst)) ")
+  proof(cases "(\<exists> d. x64_decode 0 l = Some(5, Pcall_i d))")
     case True
-    have c0_0:"update_l_jump (num,off,l) l_pc1 l_jump1 = l_jump1@[(int ?len, of_nat ?len+off)]" using True b0 update_l_jump_def by simp 
+    then show ?thesis using True an by force
+  next
+    case False
+    have b5:"\<not>(\<exists> d. x64_decode 0 l = Some(5, Pcall_i d))" using False by simp
+    then show ?thesis
+    proof(cases "(\<exists> src dst. x64_decode 0 l = Some(3, Pcmpq_rr src dst)) ")
+      case True
+      have c0_0:"update_l_jump (num,off,l) l_pc1 l_jump1 = l_jump1@[(int ?len, of_nat ?len+off)]" using True b0 update_l_jump_def using b5 True by auto
+      hence c0_1:"jitflat_bpf ((num,off,l)#?xs) (l1,l_pc1,l_jump1) = (
+          jitflat_bpf ?xs (l1@l,l_pc1@[(of_nat (length l1),num)],l_jump1@[(int ?len, of_nat ?len+off)]))" 
+        using b0 by presburger  
+      have "\<exists> l1' l_pc1' l_jump1'. jitflat_bpf [(num,off,l)] (l1,l_pc1,l_jump1) = (l1',l_pc1',l_jump1') \<and> jitflat_bpf ?xs (l1',l_pc1',l_jump1') = (l_bin,l_pc,l_jump)" 
+        using jitflat_bpf_induct a0 a7 by presburger 
+      then obtain l1' l_pc1' l_jump1' where c0:"jitflat_bpf [(num,off,l)] (l1,l_pc1,l_jump1) = (l1',l_pc1',l_jump1') \<and> jitflat_bpf ?xs (l1',l_pc1',l_jump1') = (l_bin,l_pc,l_jump)" by auto
+      hence c1:"l_jump1' = l_jump1@[(int ?len, of_nat ?len+off)]" using c0 c0_1 c0_0 by simp
+      hence "list_in_list (l_jump1@[(int ?len, of_nat ?len+off)]) 0 l_jump" using a0 a7 not_change_prefix_l_jump b1_1 c1 c0 by blast
+      hence "list_in_list [(int ?len, of_nat ?len+off)] (length l_jump1) l_jump" by (simp add: list_in_list_concat) 
+      hence "(int ?len, of_nat ?len+off) \<in> set l_jump" sorry (*using list_in_list_implies_set_relation by metis*)
+      hence "npc = off + of_nat ?len+pc" using a4 a2 b1 b2 eq_key_imp_eq_value by (metis add.commute add.right_neutral) 
+      then show ?thesis by simp
+    next
+      case False      
+      then show ?thesis using an b5 by fastforce 
+    qed
+  qed  
+qed
+  
+
+
+lemma flattern_jump_index_easy_2:
+  "jitflat_bpf lt (l1,l_pc1,l_jump1) = (l_bin,l_pc,l_jump) \<Longrightarrow>
+  lt!(unat pc) = (num,off,l) \<Longrightarrow>
+  (\<exists> d. x64_decode 0 l = Some(5, Pcall_i d)) \<Longrightarrow>
+  find_target_pc_in_l_pc l_jump (of_nat(length(l_pc1))+uint pc) = Some npc \<Longrightarrow>
+  lt \<noteq> [] \<Longrightarrow>
+  pc = 0 \<Longrightarrow>
+  distinct (map fst l_jump1) \<Longrightarrow>
+  is_increase_list l_jump1 l_pc1 \<Longrightarrow>
+  npc = off"
+proof-
+  assume a0:"jitflat_bpf lt (l1,l_pc1,l_jump1) = (l_bin,l_pc,l_jump)" and
+  a1:"lt!(unat pc) = (num,off,l)" and
+  a2:"find_target_pc_in_l_pc l_jump (int(length(l_pc1))+uint pc) = Some npc" and
+  a3:"lt \<noteq> []" and
+  a4:"pc = 0" and
+  a5:"distinct (map fst l_jump1)" and
+  a6:"is_increase_list l_jump1 l_pc1" and
+  an:"(\<exists> d. x64_decode 0 l = Some(5, Pcall_i d))"
+  let "?xs" = "tl lt"
+  let "?len" = "(length(l_pc1))"
+  have a7:"(num,off,l)#?xs = lt" using a1 a3 a4
+    by (metis list.collapse nth_Cons_0 unat_0) 
+  have b0:"jitflat_bpf ((num,off,l)#?xs) (l1,l_pc1,l_jump1) = (
+  let curr_pc = of_nat (length l1) in 
+  let l_jump' = update_l_jump (num,off,l) l_pc1 l_jump1 in
+      jitflat_bpf ?xs (
+        l1@l,
+        l_pc1@[(curr_pc,num)],
+        l_jump'))" using a0 a4 by auto 
+  have b1_1:"l_jump \<noteq> []" using a2 by force 
+  have b1:"distinct (map fst l_jump)" using l_jump_is_distinct a0 a5 a6 by blast
+  have "int ?len = (int(length(l_pc1))+uint pc)" using a4 by simp
+  hence b2:"(int ?len,npc) \<in> set l_jump" using a2 a4 b1 search_l_jump by auto 
+   (* by (metis bot_nat_0.extremum_strict in_set_conv_nth list.size(3) list_in_list.simps(1) list_in_list.simps(2) list_in_list_implies_set_relation) *)
+  have b3:"update_l_jump (num,off,l) l_pc l_jump = (
+  if (\<exists> d. x64_decode 0 l = Some(5, Pcall_i d)) then l_jump@ [(of_nat (length l_pc), off)]
+  else if (\<exists> src dst. x64_decode 0 l = Some(3, Pcmpq_rr src dst)) then l_jump@ [(of_nat (length l_pc), of_nat (length l_pc) + off)]
+  else l_jump)" 
+    apply(unfold update_l_jump_def Let_def,simp_all) done
+  have b4:"l_jump \<noteq> []" using a2 by auto
+  thus ?thesis
+  proof(cases "(\<exists> d. x64_decode 0 l = Some(5, Pcall_i d))")
+    case True
+    have c0_0:"update_l_jump (num,off,l) l_pc1 l_jump1 = l_jump1@[(int ?len, off)]" using True b0 update_l_jump_def using True by auto
     hence c0_1:"jitflat_bpf ((num,off,l)#?xs) (l1,l_pc1,l_jump1) = (
-        jitflat_bpf ?xs (l1@l,l_pc1@[(of_nat (length l1),num)],l_jump1@[(int ?len, of_nat ?len+off)]))" 
+        jitflat_bpf ?xs (l1@l,l_pc1@[(of_nat (length l1),num)],l_jump1@[(int ?len, off)]))" 
       using b0 by presburger  
     have "\<exists> l1' l_pc1' l_jump1'. jitflat_bpf [(num,off,l)] (l1,l_pc1,l_jump1) = (l1',l_pc1',l_jump1') \<and> jitflat_bpf ?xs (l1',l_pc1',l_jump1') = (l_bin,l_pc,l_jump)" 
       using jitflat_bpf_induct a0 a7 by presburger 
     then obtain l1' l_pc1' l_jump1' where c0:"jitflat_bpf [(num,off,l)] (l1,l_pc1,l_jump1) = (l1',l_pc1',l_jump1') \<and> jitflat_bpf ?xs (l1',l_pc1',l_jump1') = (l_bin,l_pc,l_jump)" by auto
-    hence c1:"l_jump1' = l_jump1@[(int ?len, of_nat ?len+off)]" using c0 c0_1 c0_0 by simp
-    hence "list_in_list (l_jump1@[(int ?len, of_nat ?len+off)]) 0 l_jump" using a0 a7 not_change_prefix_l_jump b1_1 c1 c0 by blast
-    hence "list_in_list [(int ?len, of_nat ?len+off)] (length l_jump1) l_jump" by (simp add: list_in_list_concat) 
-    hence "(int ?len, of_nat ?len+off) \<in> set l_jump" sorry (*using list_in_list_implies_set_relation by metis*)
-    hence "npc = off + of_nat ?len+pc" using a4 a2 b1 b2 eq_key_imp_eq_value by (metis add.commute add.right_neutral) 
-    then show ?thesis by simp
+    hence c1:"l_jump1' = l_jump1@[(int ?len, off)]" using c0 c0_1 c0_0 by simp
+    hence "list_in_list (l_jump1@[(int ?len, off)]) 0 l_jump" using a0 a7 not_change_prefix_l_jump b1_1 c1 c0 by blast
+    hence "list_in_list [(int ?len, off)] (length l_jump1) l_jump" by (simp add: list_in_list_concat) 
+    hence "(int ?len, off) \<in> set l_jump" sorry (*using list_in_list_implies_set_relation by metis*)
+    hence "npc = off " using a4 a2 b1 b2 eq_key_imp_eq_value by simp
+    then show ?thesis using True by force
   next
     case False
-    have "update_l_jump (num,off,l) l_pc1 l_jump1 = l_jump1" using False b0 update_l_jump_def by simp
-    hence "jitflat_bpf ((num,off,l)#?xs) (l1,l_pc1,l_jump1) = jitflat_bpf ?xs (l1@l,l_pc1@[(of_nat (length l1),num)],l_jump1)"  using b0 init_second_layer_def by fastforce
-    hence "\<not>(\<exists> x. x \<in> set l_jump \<and> fst x = (int ?len+uint pc))" using b4 a3 a0 l_jump_elem_increases a3 a6 is_increase_list_def a6 sorry
-    hence "find_target_pc_in_l_pc l_jump (int ?len+uint pc) = None" using a4 b2 by auto
-    then show ?thesis using a2 by fastforce 
-  qed
+    have b5:"\<not>(\<exists> d. x64_decode 0 l = Some(5, Pcall_i d))" using False by simp
+    then show ?thesis using an by force
+  qed  
 qed
-
-lemma flattern_jump_index:
+  
+lemma flattern_jump_index_2:
   "jitflat_bpf lt (l1,l_pc1,l_jump1) = (l_bin,l_pc,l_jump) \<Longrightarrow>
   lt!(unat pc) = (num,off,l) \<Longrightarrow>
+  distinct (map fst l_jump1) \<Longrightarrow>
+  unat pc < length lt \<and> unat pc \<ge> 0 \<Longrightarrow>
+  (\<exists> d. x64_decode 0 l = Some(5, Pcall_i d)) \<Longrightarrow>
+  is_increase_list l_jump1 l_pc1 \<Longrightarrow>
+  find_target_pc_in_l_pc l_jump (of_nat (length l_pc1) + uint pc) = Some npc \<longrightarrow> npc = off"
+  proof(induct lt arbitrary: l1 l_pc1 l_jump1 l_bin l_pc l_jump pc num off l npc)
+    case Nil
+    then show ?case by simp
+  next
+    case (Cons a lt)
+    assume assm0:"jitflat_bpf (a#lt) (l1,l_pc1,l_jump1) = (l_bin,l_pc,l_jump)" and
+      assm1:"(a#lt)!(unat pc) = (num,off,l)" and
+      assm2:"distinct (map fst l_jump1)" and
+      assm3:"unat pc < length (a#lt) \<and> unat pc \<ge> 0" and
+      assm5:"is_increase_list l_jump1 l_pc1" and
+      assm6:"(\<exists> d. x64_decode 0 l = Some(5, Pcall_i d))"
+    have a0:"unat pc = 0 \<or> unat pc \<ge> 1" by auto
+      show ?case
+      proof(cases "unat pc = 0")
+        case True
+        then show ?thesis 
+          using flattern_jump_index_easy_1 flattern_jump_index_easy_2 True assm0 assm1 assm2 assm3 unat_eq_zero init_second_layer_def
+          using Cons.prems(3) assm0 assm1 unat_eq_zero assm5 assm6 by (metis neq_Nil_conv) 
+      next
+        case False
+        have a1:"pc \<ge>1" using False a0 linorder_le_less_linear by force 
+        let "?pc" = "pc -1"
+        have b1:"unat ?pc < length lt \<and> (0::nat) \<le> unat ?pc" using assm3 a1 False unat_sub by fastforce 
+        let "?x" = "tl lt"
+        have b2:"lt ! (unat ?pc) = (num, off, l)" using assm1 False by (simp add: a1 unat_sub)      
+
+        have "\<exists> l2' l_pc2' l_jump2'. jitflat_bpf [a] (l1,l_pc1,l_jump1) = (l2',l_pc2',l_jump2') \<and> jitflat_bpf lt (l2',l_pc2',l_jump2') = (l_bin,l_pc,l_jump)" 
+          using jitflat_bpf_induct assm0 by blast 
+        then obtain l2' l_pc2' l_jump2' where b3_1:"jitflat_bpf [a] (l1,l_pc1,l_jump1) = (l2',l_pc2',l_jump2') \<and> jitflat_bpf lt (l2',l_pc2',l_jump2') = (l_bin,l_pc,l_jump)" by auto
+       
+        have "distinct (map fst l_jump2')" using l_jump_is_distinct b3_1 assm0 assm2  assm5 by blast
+        hence b4:"find_target_pc_in_l_pc l_jump ((of_nat (length l_pc2'))+uint ?pc) = Some npc \<longrightarrow> npc = off" 
+          using Cons b1 b2 b3_1 l_jump_elem_increases by blast 
+        have b5:"length l_pc2' = length l_pc1 + 1" using b3_1 l_pc_length_prop by force
+        
+        have "find_target_pc_in_l_pc l_jump ((of_nat (length l_pc1))+uint pc) = Some npc \<longrightarrow> npc = off" 
+          using b4 b5 by (smt (verit, best) a1 add.commute diff_add_cancel group_cancel.add2 of_nat_1 of_nat_add uint_sub_lem unsigned_1 word_less_eq_iff_unsigned) 
+        then show ?thesis by force 
+      qed
+    qed
+
+
+lemma flattern_jump_index_1:
+  "jitflat_bpf lt (l1,l_pc1,l_jump1) = (l_bin,l_pc,l_jump) \<Longrightarrow>
+  lt!(unat pc) = (num,off,l) \<Longrightarrow>
+  (\<exists> src dst. x64_decode 0 l = Some(3, Pcmpq_rr src dst)) \<Longrightarrow>
   distinct (map fst l_jump1) \<Longrightarrow>
   unat pc < length lt \<and> unat pc \<ge> 0  \<Longrightarrow>
   is_increase_list l_jump1 l_pc1 \<Longrightarrow>
@@ -219,14 +392,15 @@ lemma flattern_jump_index:
       assm1:"(a#lt)!(unat pc) = (num,off,l)" and
       assm2:"distinct (map fst l_jump1)" and
       assm3:"unat pc < length (a#lt) \<and> unat pc \<ge> 0" and
-      assm5:"is_increase_list l_jump1 l_pc1"
+      assm5:"is_increase_list l_jump1 l_pc1" and
+      assm6:"(\<exists> src dst. x64_decode 0 l = Some(3, Pcmpq_rr src dst))"
     have a0:"unat pc = 0 \<or> unat pc \<ge> 1" by auto
       show ?case
       proof(cases "unat pc = 0")
         case True
         then show ?thesis 
-          using flattern_jump_index_easy True assm0 assm1 assm2 assm3 unat_eq_zero init_second_layer_def
-          using Cons.prems(3) assm0 assm1 flattern_jump_index_easy unat_eq_zero assm5 by blast
+          using flattern_jump_index_easy_1 flattern_jump_index_easy_1 True assm0 assm1 assm2 assm3 unat_eq_zero init_second_layer_def
+          using Cons.prems(3) assm0 assm1 assm6 unat_eq_zero assm5 by (metis (mono_tags, lifting) list.discI)
       next
         case False
         have a1:"pc \<ge>1" using False a0 linorder_le_less_linear by force 
