theory/JITFlattern_prob.thy
@@ -438,7 +438,7 @@ lemma not_cmp_insn:"l\<noteq>[] \<Longrightarrow> l!(pc+1) \<noteq> 0x39 \<Longr
 
 lemma x64_bin_is_sequential_x64_decode2:
   "jitper insns = Some lt \<Longrightarrow> 
-  lt!(unat pc) = (num,off,l_bin0) \<Longrightarrow>
+  lt!(unat pc) = (num,off,l) \<Longrightarrow>
   unat pc < length lt \<and> unat pc \<ge> 0 \<Longrightarrow>
   x64_decode 0 l \<noteq> None \<Longrightarrow> 
   x64_decode 0 l \<noteq> Some (1,Pret) \<Longrightarrow> 
